omni/OmniSmall.v
@@ -6,16 +6,24 @@
 Set Implicit Arguments.
 Require Export Syntax.
 
-(* ########################################################### *)
-(* ########################################################### *)
-(* ########################################################### *)
-(** * Omni-Small-Step *)
+Implicit Types f : var.
+Implicit Types b : bool.
+Implicit Types p : loc.
+Implicit Types n : int.
+Implicit Types v w r vf vx : val.
+Implicit Types t : trm.
+Implicit Types s : state.
 
 Implicit Types P : state->trm->Prop.
 
 
 (* ########################################################### *)
-(** ** Definition of Omni-Small-Step *)
+(* ########################################################### *)
+(* ########################################################### *)
+(** * Definitions *)
+
+(* ########################################################### *)
+(** ** Omni-Small-Step Judgment *)
 
 (** [omnismall s t P] asserts that a configuration [(s,t)] can
     take a step, and that for any step it takes it reaches a
@@ -69,64 +77,7 @@ Inductive omnismall : state -> trm -> (state->trm->Prop) -> Prop :=
 
 
 (* ########################################################### *)
-(** ** Equivalence of Omni-Small-Step with Standard Small Step *)
-
-Section OmnismallEquiv.
-Hint Constructors step.
-
-(* Characterization lemma (omni-small-step-iff-progress-and-correct). *)
-
-Lemma omnismall_iff_step_st : forall s t P,
-       omnismall s t P
-  <-> (   (exists s' t', step s t s' t')
-       /\ (forall s' t', step s t s' t' -> P s' t')).
-Proof using.
-  iff M.
-  { induction M.
-    { forwards (R&M1): IHM. split.
-      { destruct R as (s'&t'&S). exists. applys step_let_ctx S. }
-      { intros s' t' S. inverts S as.
-        { rename H into IHM1. introv S1. lets K1: M1 S1. applys IHM1 K1. }
-        { destruct R as (s''&t''&S'). false* step_val_inv. } } }
-    { split*. { intros s' t' S. inverts S as; try false_invert. { auto. } } }
-    { split*. { intros s' t' S. inverts S as; try false_invert.
-                { inverts* TEMP. } } }
-    { split*. { intros s' t' S. inverts S as; try false_invert. { auto. } } }
-    { split*. { intros s' t' S. inverts S as; try false_invert. { auto. } } }
-    { split*. { intros s' t' S. inverts S as; try false_invert. { auto. } } }
-    { split.
-       { exists. applys step_rand 0. math. }
-       { intros s' t' S. inverts S as; try false_invert.
-         { intros R. inverts R. auto. } } }
-    { split.
-       { forwards~ (p&F&N): (exists_fresh null s).
-         exists. applys* step_ref p. }
-       { intros s' t' S. inverts S as; try false_invert. { auto. } } }
-    { split*. { intros s' t' S. inverts S as; try false_invert. { auto. } } }
-    { split*. { intros s' t' S. inverts S as; try false_invert. { auto. } } }
-    { split*. { intros s' t' S. inverts S as; try false_invert. { auto. } } } }
-  { destruct M as (R&M). destruct R as (s'&t'&S).
-    gen P. induction S; intros.
-    { rename S into S1. applys omnismall_let_ctx (step s1 t1).
-      { applys IHS. auto. }
-      { intros s' t' S1'. applys M. applys step_let_ctx S1'. } }
-    { applys* omnismall_fix. }
-    { applys* omnismall_app_fix. }
-    { applys* omnismall_if. }
-    { applys* omnismall_let. }
-    { applys* omnismall_div. }
-    { applys* omnismall_rand. math. }
-    { applys* omnismall_ref. }
-    { applys* omnismall_get. }
-    { applys* omnismall_set. }
-    { applys* omnismall_free. } }
-Qed.
-
-End OmnismallEquiv.
-
-
-(* ########################################################### *)
-(** ** Eventually Judgment *)
+(** ** Eventually Judgment with Omni-Small-Step *)
 
 (** [eventually s t P] asserts that all executions starting from [(s,t)]
     eventually reach a configuration [(s',t')] satisfying the predicate [P]. *)
@@ -141,6 +92,48 @@ Inductive eventually : state->trm->(state->trm->Prop)->Prop :=
       omnismall s t P1 ->
       (forall s' t', P1 s' t' -> eventually s' t' P) ->
       eventually s t P.
+
+
+
+(* ########################################################### *)
+(* ########################################################### *)
+(* ########################################################### *)
+(** * Properties *)
+
+(* ########################################################### *)
+(** ** Chained Rules and Cut Rules *)
+
+(** The cut rule for [eventually]. *)
+
+Lemma eventually_cut : forall s t P1 P2,
+  eventually s t P1 ->
+  (forall s' t', P1 s' t' -> eventually s' t' P2) ->
+  eventually s t P2.
+Proof using.
+  introv M HK. induction M.
+  { rename H into M1. applys HK M1. }
+  { rename H into R, H0 into M1, H1 into IH1.
+    applys eventually_step R. intros s' t' S.
+    applys IH1 S HK. }
+Qed.
+
+(** One-Step Chained rule [eventually]. *)
+
+Lemma eventually_step_chained : forall s t P,
+  omnismall s t (fun s' t' => eventually s' t' P) ->
+  eventually s t P.
+Proof using. introv M. applys* eventually_step M. Qed.
+
+(** Chained rule for [eventually]. *)
+
+Lemma eventually_cut_chained : forall s t P,
+  eventually s t (fun s' t' => eventually s' t' P) ->
+  eventually s t P.
+Proof using. introv M. applys* eventually_cut M. Qed.
+
+
+(* ########################################################### *)
+(** ** Reformulation of the Eventually Judgment without Omni-Small-Step *)
 
 (** Alternative definition of [eventually], with respect to standard small-step.
     (eventually-step-using-standard-small-step) *)
@@ -173,76 +166,3 @@ Proof using.
       { autos*. } } }
 Qed.
 
-(** Chained rule for [eventually_step]. *)
-
-Lemma eventually_step_chained : forall s t P,
-  omnismall s t (fun s' t' => eventually s' t' P) ->
-  eventually s t P.
-Proof using. introv M. applys* eventually_step M. Qed.
-
-(** The cut rule for [eventually]. *)
-
-Lemma eventually_cut : forall s t P1 P2,
-  eventually s t P1 ->
-  (forall s' t', P1 s' t' -> eventually s' t' P2) ->
-  eventually s t P2.
-Proof using.
-  introv M HK. induction M.
-  { rename H into M1. applys HK M1. }
-  { rename H into R, H0 into M1, H1 into IH1.
-    applys eventually_step R. intros s' t' S.
-    applys IH1 S HK. }
-Qed.
-
-(** Chained rule for [eventually_cut]. *)
-
-Lemma eventually_cut_chained : forall s t P,
-  eventually s t (fun s' t' => eventually s' t' P) ->
-  eventually s t P.
-Proof using. introv M. applys* eventually_cut M. Qed.
-
-
-(* ########################################################### *)
-(** ** Inductive Small-Step Judgment *)
-
-(** The judgment [bigsmall] introduced in this section helps
-    carrying out several proofs of equivalence---see the next
-    section. *)
-
-(** Viewing postconditions as predicates over configurations *)
-
-Definition pred_of_post (Q:val->hprop) : state->trm->Prop :=
-  fun s' t' => exists v', t' = trm_val v' /\ Q v' s'.
-
-(** We introduce the inductive small-step judgment, as it is useful
-    to relate Omni-Small-Step with Omni-Big-Step.
-
-    [bigsmall s t Q] asserts that executions of [(t,s)] terminate,
-    and the results satisfy the postcondition [Q]. *)
-
-Inductive bigsmall : state->trm->(val->hprop)->Prop :=
-  | bigsmall_val : forall s v Q,
-      Q v s ->
-      bigsmall s v Q
-  | bigsmall_step : forall s t Q,
-      (exists s' t', step s t s' t') ->
-      (forall s' t', step s t s' t' -> bigsmall s' t' Q) ->
-      bigsmall s t Q.
-
-(** [bigsmall] is equivalent to [eventually]. *)
-
-Lemma bigsmall_iff_eventually : forall s t Q,
-  bigsmall s t Q <-> eventually s t (pred_of_post Q).
-Proof using.
-  rewrite eventually_eq_eventually'.
-  iff M.
-  { induction M.
-    { applys eventually'_here. hnf. exists*. }
-    { rename H into R, H0 into M1, H1 into IH1.
-      applys eventually'_step R. applys IH1. } }
-  { gen_eq C: (pred_of_post Q). induction M; intros; subst.
-    { destruct H as (v'&->&Hv'). applys bigsmall_val Hv'. }
-    { rename H into R, H0 into M1, H1 into IH1.
-      applys bigsmall_step R.
-      intros s' t' S. applys* IH1 S. } }
-Qed.
